Gvf_Aux.thy
@@ -1,0 +1,10 @@
+(*
+  Goal verification framework
+    - Auxiliary 
+*)  
+                            
+theory Gvf_Aux imports Main begin
+
+(* ToDo *)
+
+end
